src/program_proof/mvcc/txn_delete.v
@@ -6,12 +6,14 @@ Context `{!heapGS Σ, !mvcc_ghostG Σ}.
 (*****************************************************************)
 (* func (txn *Txn) Delete(key uint64) bool                       *)
 (*****************************************************************)
-Theorem wp_txn__Delete txn (k : u64) γ :
-  {{{ own_txn txn γ }}}
+Theorem wp_txn__Delete txn (k : u64) dbv γ τ :
+  {{{ own_txn txn γ τ ∗ txnmap_ptsto τ k dbv }}}
     Txn__Delete #txn #k
-  {{{ (ok : bool), RET #ok; own_txn txn γ }}}.
+  {{{ (ok : bool), RET #ok;
+      own_txn txn γ τ ∗ txnmap_ptsto τ k Nil
+  }}}.
 Proof.
-  iIntros (Φ) "Htxn HΦ".
+  iIntros (Φ) "[Htxn Hptsto] HΦ".
   iNamed "Htxn".
   iNamed "Himpl".
   wp_call.
@@ -25,13 +27,21 @@ Proof.
   wp_apply (wp_wrbuf__Delete with "HwrbufRP").
   iIntros "HwrbufRP".
   wp_pures.
+  iMod (txnmap_update Nil with "Htxnmap Hptsto") as "[Htxnmap Hptsto]".
 
   (***********************************************************)
   (* return true                                             *)
   (***********************************************************)
   iModIntro.
   iApply "HΦ".
-  eauto 20 with iFrame.
+  iSplitR "Hptsto".
+  { unfold own_txn.
+    rewrite insert_union_l.
+    set mods' := (<[ _ := _ ]> mods).
+    iExists _, view, mods'.
+    eauto 20 with iFrame.
+  }
+  iFrame.
 Qed.
 
 End program.
