src/program_proof/mvcc/txn_get.v
@@ -6,43 +6,51 @@ Context `{!heapGS Σ, !mvcc_ghostG Σ}.
 (*****************************************************************)
 (* func (txn *Txn) Get(key uint64) (uint64, bool)                *)
 (*****************************************************************)
-Theorem wp_txn__Get txn (k : u64) γ :
-  {{{ own_txn txn γ }}}
+Theorem wp_txn__Get txn (k : u64) dbv γ τ :
+  {{{ own_txn txn γ τ ∗ txnmap_ptsto τ k dbv }}}
     Txn__Get #txn #k
-  {{{ (v : u64) (found : bool), RET (#v, #found); own_txn txn γ }}}.
+  {{{ (v : u64) (found : bool), RET (#v, #found);
+      own_txn txn γ τ ∗ txnmap_ptsto τ k dbv ∗ ⌜dbv = to_dbval found v⌝
+  }}}.
 Proof.
-  iIntros (Φ) "Htxn HΦ".
+  iIntros (Φ) "[Htxn Hptsto] HΦ".
   iNamed "Htxn".
   iNamed "Himpl".
   wp_call.
 
   (***********************************************************)
   (* wrbuf := txn.wrbuf                                      *)
-  (* valb, del, found := wrbuf.Lookup(key)                   *)
+  (* valb, wr, found := wrbuf.Lookup(key)                    *)
   (***********************************************************)
   wp_loadField.
   wp_pures.
   wp_apply (wp_wrbuf__Lookup with "HwrbufRP").
-  iIntros (v d ok) "[HwrbufRP %HLookup]".
+  iIntros (v d ok) "[HwrbufRP %Hlookup]".
   wp_pures.
 
   (***********************************************************)
   (* if found {                                              *)
-  (*     return valb, !del                                   *)
+  (*     return valb, wr                                     *)
   (* }                                                       *)
   (***********************************************************)
-  unfold spec_wrbuf__Lookup in HLookup.
+  unfold spec_wrbuf__Lookup in Hlookup.
   wp_if_destruct.
   { wp_pures.
     iModIntro.
     iApply "HΦ".
-    eauto 20 with iFrame.
+    iDestruct (txnmap_lookup with "Htxnmap Hptsto") as "%Hlookup'".
+    apply (lookup_union_Some_l _ view) in Hlookup.
+    rewrite Hlookup' in Hlookup.
+    inversion_clear Hlookup.
+    iSplitR "Hptsto".
+    { eauto 20 with iFrame. }
+    by iFrame.
   }
 
   (***********************************************************)
   (* idx := txn.idx                                          *)
   (* tuple := idx.GetTuple(key)                              *)
-  (* val, ret := tuple.ReadVersion(txn.tid)                  *)
+  (* val, found := tuple.ReadVersion(txn.tid)                *)
   (***********************************************************)
   wp_loadField.
   wp_pures.
@@ -52,7 +60,7 @@ Proof.
   wp_loadField.
   wp_apply (wp_tuple__ReadVersion with "HtupleRI [Hactive]").
   { unfold active_tid. eauto with iFrame. }
-  iIntros (val ret latch) "[Hactive [Hlocked Hread]]".
+  iIntros (val found latch) "[Hactive [Hlocked Hread]]".
   wp_pures.
 
   (***********************************************************)
@@ -67,12 +75,39 @@ Proof.
   iExists future.
   iFrame "Hproph".
   iIntros "(%future' & %Hresolve & Hproph)".
+  (* Extend the physical tuple. *)
+  iMod (tuple_read_safe with "Hkeys Hcmt Hread") as "(Hkeys & Hcmt & Htuple & Hptuple)"; first set_solver.
+  (* Deduce eq between logical and physical read. *)
   iDestruct (big_sepS_elem_of_acc _ _ k with "Hkeys") as "[Hkey Hkeys]"; first set_solver.
-  iMod (tuple_read_safe with "[$Hkey $Hcmt] Hread") as "[[Hkey Hcmt] Htuple]"; first set_solver.
+  iDestruct (txnmap_lookup with "Htxnmap Hptsto") as "%Hlookup'".
+  rewrite lookup_union_r in Hlookup'; last auto.
+  iDestruct (big_sepM_lookup_acc with "Hltuples") as "[Hltuple Hltuples]"; first apply Hlookup'.
+  iDestruct (ltuple_ptuple_ptsto_eq with "[Hkey] Hltuple Hptuple") as "%Heq".
+  { iNamed "Hkey".
+    unfold tuple_auth_prefix.
+    unfold tuple_mods_rel in Htmrel.
+    destruct Htmrel as (diff & _ & [H _]).
+    do 2 iExists _.
+    iFrame.
+    iPureIntro.
+    by exists diff.
+  }
+  (* Close things. *)
   iDestruct ("Hkeys" with "Hkey") as "Hkeys".
+  iDestruct ("Hltuples" with "Hltuple") as "Hltuples".
   iMod "Hclose".
   iMod ("HinvC" with "[Hproph Hm Hkeys Hcmt Hnca Hfa Hfci Hfcc]") as "_".
-  { (* Close the inv. *) admit. }
+  { (* Close the inv. *)
+    iNext. unfold mvcc_inv_sst_def.
+    do 6 iExists _.
+    iExists (past ++ [EvRead tid k]), future'.
+    iDestruct (nca_inv_head_read with "Hnca") as "Hnca"; first apply Hresolve.
+    iDestruct (fa_inv_head_read  with "Hfa")  as "Hfa";  first apply Hresolve.
+    iDestruct (fci_inv_head_read with "Hfci") as "Hfci"; first apply Hresolve.
+    iDestruct (fcc_inv_head_read with "Hfcc") as "Hfcc"; first apply Hresolve.
+    iDestruct (cmt_inv_head_read with "Hcmt") as "Hcmt"; first apply Hresolve.
+    iFrame.
+  }
   iModIntro.
   iIntros "_".
   wp_pures.
@@ -84,13 +119,18 @@ Proof.
   wp_pures.
 
   (***********************************************************)
-  (* return val, ret == common.RET_SUCCESS                   *)
+  (* return val, found                                       *)
   (***********************************************************)
   iModIntro.
   iApply "HΦ".
-  do 7 iExists _.
-  iFrame "Hactive".
-  iFrameNamed.
-Admitted.
+  iSplitR "Hptsto".
+  { do 3 iExists _.
+    iFrame "Hltuples Htxnmap".
+    do 5 iExists _.
+    iFrame "Hactive Htid Hsid Hwrbuf HwrbufRP".
+    by iFrame "#".
+  }
+  by iFrame "Hptsto".
+Qed.
 
 End program.
