src/program_proof/mvcc/txn_put.v
@@ -6,12 +6,13 @@ Context `{!heapGS Σ, !mvcc_ghostG Σ}.
 (*****************************************************************)
 (* func (txn *Txn) Put(key, val uint64)                          *)
 (*****************************************************************)
-Theorem wp_txn__Put txn (k : u64) (v : u64) γ :
-  {{{ own_txn txn γ }}}
+Theorem wp_txn__Put txn (k : u64) dbv v γ τ :
+  {{{ own_txn txn γ τ ∗ txnmap_ptsto τ k dbv }}}
     Txn__Put #txn #k #v
-  {{{ RET #(); own_txn txn γ }}}.
+  {{{ RET #();
+      own_txn txn γ τ ∗ txnmap_ptsto τ k (Value v) }}}.
 Proof.
-  iIntros (Φ) "Htxn HΦ".
+  iIntros (Φ) "[Htxn Hptsto] HΦ".
   iNamed "Htxn".
   iNamed "Himpl".
   wp_call.
@@ -25,10 +26,18 @@ Proof.
   wp_apply (wp_wrbuf__Put with "HwrbufRP").
   iIntros "HwrbufRP".
   wp_pures.
+  iMod (txnmap_update (Value v) with "Htxnmap Hptsto") as "[Htxnmap Hptsto]".
 
   iModIntro.
   iApply "HΦ".
-  eauto 20 with iFrame.
+  iSplitR "Hptsto".
+  { unfold own_txn.
+    rewrite insert_union_l.
+    set mods' := (<[ _ := _ ]> mods).
+    iExists _, view, mods'.
+    eauto 20 with iFrame.
+  }
+  iFrame.
 Qed.
 
 End program.
